paramDirect.v
@@ -83,13 +83,15 @@ Definition PiABType@{i it j jt}
 forall (a1 : A1) (a2 : A2) (p : A_R a1 a2), B_R a1 a2 p (f1 a1) (f2 a2)).
 *)
 
+
+
   
 Definition PiABType (Asp Bsp:bool) (a1:V)
   (A1 A2 A_R B1 B2 B_R : STerm) : STerm :=
 let allVars := flat_map all_vars ([A1; A2; B1; B2; A_R; B_R]) in
 let f1l : list V := 
   let cl :(decSubtype (fun n : N => (n < 3)%N)) := 
-    exist (fun t : N => decide (t < 3) = true) 0 eq_refl in
+    userVar in
     (@freshVars V (decSubtype (fun n : N => (n < 3)%N)) _ 
       1 (Some cl) (a1::allVars) [changeVarName a1 "ff"]) in
 match f1l with
